src/Backtranslation.v
@@ -1,6 +1,6 @@
 (**************************************************************************
-* Backtranslation from Ahmed & Blume ICFP 2011                            *
-* William J. Bowman, Phillip Mates & James T. Perconti                    *
+* Backtranslation from Ahmed +&+ Blume ICFP 2011                            *
+* William J. Bowman, Phillip Mates +&+ James T. Perconti                    *
 ***************************************************************************)
 Require Import Core_Definitions Source_Definitions Target_Definitions
                LibWfenv Cps_Trans_Definitions Multi_Definitions.
@@ -15,7 +15,7 @@ Inductive subformula : env_term -> trm -> typ -> Prop :=
 | sf_s_false : forall G,
     wfenv trans_type G -> subformula G s_trm_false s_typ_bool
 | sf_s_abs : forall L G e s1 s2,
-    (forall x, x \notinLN L -> subformula (G & x ~ s1) (s_open_ee_var e x) s2) ->
+    (forall x, x \notinLN L -> subformula (G +&+ x ~ s1) (s_open_ee_var e x) s2) ->
     (s_type s1) ->
     subformula G (s_trm_abs s1 e) (s_typ_arrow s1 s2)
 | sf_s_if : forall G e1 e2 e3 s,
@@ -36,7 +36,7 @@ Inductive subformula : env_term -> trm -> typ -> Prop :=
     wfenv trans_type G ->
     (* The follow may be wrong, we need to add the first projection of the functions argument to the context *)
     (forall x, x \notinLN L ->
-      subformula (G & x ~ (t_typ_pair (s1+) (t_typ_arrow (s2+) (s2+)))) (t_open_ee_var m x) (s2+)) ->
+      subformula (G +&+ x ~ (t_typ_pair (s1+) (t_typ_arrow (s2+) (s2+)))) (t_open_ee_var m x) (s2+)) ->
     subformula G
     (* λ[α] (y,k) . let x = TS STe in (k x) *)
     (t_trm_abs (t_typ_pair (s1+) (t_typ_arrow (s2+) (t_typ_bvar 1)))
@@ -52,14 +52,14 @@ Inductive subformula : env_term -> trm -> typ -> Prop :=
 | sf_t_app : forall L G u1 u2a u2kontbody s s1 s2,
     subformula G u1 ((s_typ_arrow s1 s2)+) ->
     subformula G u2a (s1+) ->
-    (forall x, x \notinLN L -> subformula (G & x ~ (s2+)) (t_open_ee_var u2kontbody x) (s+)) ->
+    (forall x, x \notinLN L -> subformula (G +&+ x ~ (s2+)) (t_open_ee_var u2kontbody x) (s+)) ->
     subformula G (t_trm_app u1 (s+) (t_trm_pair u2a (t_trm_abs (s2+) u2kontbody))) (s+)
 (* boundary type *)
 | sf_st : forall G m s,
     subformula G m (s+) -> subformula G (s_trm_st m s) s
 | sf_ts : forall L G e m s t,
     subformula G e s ->
-    (forall x, x \notinLN L -> subformula (G & x ~ (s+)) (t_open_ee_var m x) t) ->
+    (forall x, x \notinLN L -> subformula (G +&+ x ~ (s+)) (t_open_ee_var m x) t) ->
     subformula G (t_trm_ts e s m) t.
 
 (* Partial reduction relation *)
@@ -72,7 +72,7 @@ Inductive partial_eval : env_term -> trm -> typ -> trm -> Prop :=
 | sf_s_false : forall G,
     wfenv trans_type G -> partial_eval G s_trm_false s_typ_bool s_trm_false
 | sf_s_abs : forall L G e ep s1 s2,
-    (forall x, x \notinLN L -> partial_eval (G & x ~ s1) (s_open_ee_var e x) s2 (s_open_ee_var ep x)) ->
+    (forall x, x \notinLN L -> partial_eval (G +&+ x ~ s1) (s_open_ee_var e x) s2 (s_open_ee_var ep x)) ->
     (s_type s1) ->
     partial_eval G (s_trm_abs s1 e) (s_typ_arrow s1 s2) (s_trm_abs s1 ep)
 | sf_s_if : forall G e1 e1p e2 e2p e3 e3p s,
@@ -91,7 +91,7 @@ Inductive partial_eval : env_term -> trm -> typ -> trm -> Prop :=
     wfenv trans_type G -> partial_eval G t_trm_false t_typ_bool t_trm_false
 | sf_t_abs : forall L G m mp s s1 s2,
     wfenv trans_type G ->
-    (forall y, y \notinLN L -> partial_eval (G & y ~ (s1+))
+    (forall y, y \notinLN L -> partial_eval (G +&+ y ~ (s1+))
       (t_trm_let_fst (t_trm_bvar 0)
         (t_open_ee (t_open_ee (open_te m (s2+)) t_id)) y))
       (s2+) mp) ->
@@ -113,12 +113,12 @@ Inductive partial_eval : env_term -> trm -> typ -> trm -> Prop :=
 | sf_t_app : forall L G u1 u1p u2a u2ap u2kontbody u2kontbodyp s s1 s2,
     partial_eval G u1 ((s_typ_arrow s1 s2)+) u1p ->
     partial_eval G u2a (s1+) u2ap ->
-    (forall x, x \notinLN L -> partial_eval (G & x ~ (s2+)) (t_open_ee_var u2kontbody x) (s+)) (t_open_ee_var u2kontbodyp x)->
+    (forall x, x \notinLN L -> partial_eval (G +&+ x ~ (s2+)) (t_open_ee_var u2kontbody x) (s+)) (t_open_ee_var u2kontbodyp x)->
     partial_eval G (t_trm_app u1 (s+) (t_trm_pair u2a (t_trm_abs (s2+) u2kontbody))) (s+)
 (* boundary type *)
 | sf_st : forall G m mp s,
     partial_eval G m (s+) mp -> partial_eval G (s_trm_st m s) s (s_trm_st mp s)
 | sf_ts : forall L G e ep m mp s t,
     partial_eval G e s ep ->
-    (forall x, x \notinLN L -> partial_eval (G & x ~ (s+)) (t_open_ee_var m x) t (t_open_ee_var mp x)) ->
+    (forall x, x \notinLN L -> partial_eval (G +&+ x ~ (s+)) (t_open_ee_var m x) t (t_open_ee_var mp x)) ->
     partial_eval G (t_trm_ts e s m) t (t_trm_ts ep s mp).
