src/Core_Infrastructure.v
@@ -1,7 +1,7 @@
 (***************************************************************************
 * Core Infrastructure                                                      *
-* Multilanguage present in Ahmed & Blume ICFP 2011
-* William J. Bowman, Phillip Mates & James T. Perconti                     *
+* Multilanguage present in Ahmed +&+ Blume ICFP 2011
+* William J. Bowman, Phillip Mates +&+ James T. Perconti                     *
 ***************************************************************************)
 
 Require Export Core_Definitions.
@@ -226,21 +226,21 @@ Qed.
 (* weakening for substitutions *)
 
 Lemma subst_tt_push : forall t X t' d, X \notinLN fv_tt t ->
-  subst_tt (d & X ~ t') t = subst_tt d t.
+  subst_tt (d +&+ X ~ t') t = subst_tt d t.
 Proof.
   induction t; simpl; intros; auto; try rewrite* IHt1; try rewrite* IHt2.
   rewrite get_push. cases_if*. false. auto using in_singleton_self.
 Qed.
 
 Lemma subst_te_push : forall e X t d, X \notinLN fv_te e ->
-  subst_te (d & X ~ t) e = subst_te d e.
+  subst_te (d +&+ X ~ t) e = subst_te d e.
 Proof.
   induction e; simpl; auto; intros; try rewrite* subst_tt_push;
     try rewrite* IHe; try rewrite* IHe1; try rewrite* IHe2; try rewrite* IHe3.
 Qed.
 
 Lemma subst_ee_push : forall e x e' g l, x \notinLN fv_ee l e ->
-  subst_ee l (g & x ~ e') e = subst_ee l g e.
+  subst_ee l (g +&+ x ~ e') e = subst_ee l g e.
 Proof.
   induction e; simpl; intros; auto;
     try rewrite* IHe; try rewrite* IHe1; try rewrite* IHe2; try rewrite* IHe3;
@@ -248,7 +248,7 @@ Proof.
 Qed.
 
 Lemma subst_tt_weaken : forall t X t' d d', X \notinLN fv_tt t ->
-  subst_tt (d & X ~ t' & d') t = subst_tt (d & d') t.
+  subst_tt (d +&+ X ~ t' +&+ d') t = subst_tt (d +&+ d') t.
 Proof.
   induction t; simpl; intros; auto; try rewrite* IHt1; try rewrite* IHt2.
   repeat rewrite get_concat. destruct* (get v d').
@@ -256,14 +256,14 @@ Proof.
 Qed.
 
 Lemma subst_te_weaken : forall e X t d d', X \notinLN fv_te e ->
-  subst_te (d & X ~ t & d') e = subst_te (d & d') e.
+  subst_te (d +&+ X ~ t +&+ d') e = subst_te (d +&+ d') e.
 Proof.
   induction e; simpl; auto; intros; try rewrite* subst_tt_weaken;
     try rewrite* IHe; try rewrite* IHe1; try rewrite* IHe2; try rewrite* IHe3.
 Qed.
 
 Lemma subst_ee_weaken : forall e x e' g g' l, x \notinLN fv_ee l e ->
-  subst_ee l (g & x ~ e' & g') e = subst_ee l (g & g') e.
+  subst_ee l (g +&+ x ~ e' +&+ g') e = subst_ee l (g +&+ g') e.
 Proof.
   induction e; simpl; intros; auto;
     try rewrite* IHe; try rewrite* IHe1; try rewrite* IHe2; try rewrite* IHe3;
@@ -273,13 +273,13 @@ Qed.
 
 (* exchange for substitutions *)
 
-Lemma subst_tt_exchange : forall t D1 D2 D3 D4, ok (D1 & D2 & D3 & D4) ->
-  subst_tt (D1 & D2 & D3 & D4) t = subst_tt (D1 & D3 & D2 & D4) t.
+Lemma subst_tt_exchange : forall t D1 D2 D3 D4, ok (D1 +&+ D2 +&+ D3 +&+ D4) ->
+  subst_tt (D1 +&+ D2 +&+ D3 +&+ D4) t = subst_tt (D1 +&+ D3 +&+ D2 +&+ D4) t.
 Proof.
   induction t; simpl; intros; f_equal*.
   repeat rewrite get_concat.
   case_eq (get v D1); case_eq (get v D2); case_eq (get v D3); case_eq (get v D4); intros; auto;
-  apply binds_func with (x := v) (E := D1 & D2 & D3 & D4); repeat apply* binds_concat_left_ok.
+  apply binds_func with (x := v) (E := D1 +&+ D2 +&+ D3 +&+ D4); repeat apply* binds_concat_left_ok.
 Qed.
 
 (* fv and open *)
@@ -367,7 +367,7 @@ Ltac frauto :=
               => let Fr := fresh "Fr" in assert (Fr : x \notinLN L); eauto end.
 
 (** These tactics help applying a lemma which conclusion mentions
-  an environment (E & F) in the particular case when F is empty *)
+  an environment (E +&+ F) in the particular case when F is empty *)
 
 (* TODO:
 Ltac get_env_type :=
